MicroGV

theories/microgv/invariant.v
@@ -1,6 +1,14 @@
 From diris.microgv Require Export rtypesystem.
 
-Definition linv (ρ : cfg) (v : vertex) (in_l : multiset label) : rProp :=
+(* Can we just do vertex = nat here? *)
+Definition linv (ρ : cfg) (v : nat) (in_l : multiset label) : rProp :=
+  match ρ !! v with
+  | Some (Thread e) => ⌜⌜ in_l ≡ ε ⌝⌝ ∗ rtyped0 e UnitT
+  | Some Barrier => ⌜⌜ ∃ t1 t2, in_l ≡ {[ (t1,t2) ]} ⋅ {[ (t2,t1) ]} ⌝⌝
+  | None => ⌜⌜ in_l ≡ ε ⌝⌝
+  end.
+
+(* Definition linv (ρ : cfg) (v : vertex) (in_l : multiset label) : rProp :=
   match v with
   | VThread k =>
     ⌜⌜ in_l ≡ ε ⌝⌝ ∗
@@ -10,10 +18,10 @@ Definition linv (ρ : cfg) (v : vertex) (in_l : multiset label) : rProp :=
     end
   | VBarrier k =>
     ⌜⌜ match ρ !! k with
-      | Some Barrier => ∃ t1 t2, in_l ≡ {[ (t1,t2)]} ⋅ {[ (t2,t1) ]}
+      | Some Barrier => ∃ t1 t2, in_l ≡ {[ (t1,t2) ]} ⋅ {[ (t2,t1) ]}
       | _ => in_l ≡ ε
       end ⌝⌝
-  end%I.
+  end%I. *)
 
 Global Instance lin_Proper ρ v : Proper ((≡) ==> (≡)) (linv ρ v).
 Proof. solve_proper. Qed.
@@ -42,33 +50,98 @@ Proof.
   destruct H as [ρ ρ' ρf D1 D2 i H].
   destruct H.
   - eapply inv_impl; last done.
-    iIntros ([n|n] x) "H"; smap.
+    iIntros (n x) "H". unfold linv. smap.
     iDestruct "H" as "[? H]". iFrame.
     iDestruct (replacement with "H") as (t) "[H Q]"; first done.
     iApply "Q". iApply pure_preservation; done.
   - eapply inv_impl; last done.
-    iIntros ([n|n] x) "H"; smap; iDestr "H";
+    iIntros (n x) "H". unfold linv. smap; iDestr "H";
     assert (ρf !! n = None) as -> by solve_map_disjoint; eauto.
     destruct v; simpl; iDestr "H"; simp. done.
-  - eapply (inv_alloc_lr (VThread i0) (VBarrier n) (VThread j));
+  - eapply (inv_alloc_lr i0 n j);
     last done; first apply _; first apply _.
     + naive_solver.
-    + iIntros (? ? ?) "H". simp.
-      destruct v0; simpl; smap;
-      assert (ρf !! n0 = None) as -> by solve_map_disjoint; eauto.
-    + iIntros (?) "H". simpl. smap.
+    + iIntros (? ? ?) "H". unfold linv. smap.
+    + iIntros (?) "H". unfold linv. smap.
       assert (ρf !! n = None) as -> by solve_map_disjoint; eauto.
-    + iIntros (?) "H". simpl. smap. iDestr "H".
+    + iIntros (?) "H". unfold linv. smap.
       assert (ρf !! j = None) as -> by solve_map_disjoint; eauto.
-    + iIntros (?) "H". simpl.
-      iDestr "H". rewrite lookup_union_spec lookup_singleton. simpl.
+    + iIntros (?) "H". unfold linv. smap. iDestr "H".
       iDestruct (replacement with "H") as (t) "[H Q]"; first done. simpl.
       iDestr "H". simp.
       iExists (t1,t2), (t2,t1).
       iSplitL "Q".
-      * smap. iIntros "H". iSplit; first done.
+      * iIntros "H". iSplit; first done.
         iApply "Q". simpl. eauto.
-      * smap. iSplit; eauto.
+      * iSplit; eauto.
         iIntros "Q". iSplit; eauto 10 with iFrame.
   - admit.
+Admitted.
+
+Lemma fresh2 (s : gset nat) :
+  ∃ x y, x ∉ s ∧ y ∉ s ∧ x ≠ y.
+Proof.
+  exists (fresh s), (fresh (s ∪ {[ fresh s ]})).
+  split; first apply is_fresh.
+  pose proof (is_fresh (s ∪ {[ fresh s ]})).
+  set_solver.
+Qed.
+
+Lemma cfg_fresh2 (ρ : cfg) :
+  ∃ j1 j2, ρ !! j1 = None ∧ ρ !! j2 = None ∧ j1 ≠ j2.
+Proof.
+  destruct (fresh2 (dom (gset nat) ρ)) as (j1 & j2 & H1 & H2 & H3).
+  exists j1,j2. split_and!; last done;
+  apply not_elem_of_dom; done.
+Qed.
+
+Lemma full_reachability ρ :
+  ginv ρ -> fully_reachable ρ.
+Proof.
+  unfold fully_reachable.
+  intros Hinv.
+  destruct Hinv as [g [Hwf Hinv]].
+  eapply (cgraph_ind' (λ a b l, waiting ρ a b)); [solve_proper|eauto|].
+  intros i IH1 IH2.
+  classical_right.
+  rewrite /inactive in H.
+  pose proof (Hinv i) as Q.
+  unfold linv in Q.
+  destruct (ρ !! i) eqn:E; simplify_eq. clear H.
+  destruct o.
+  - apply pure_sep_holds in Q as [Q1 Q2]. assert (Q2' := Q2).
+    eapply holds_entails in Q2; last apply pure_progress.
+    assert (ρ = {[ i := Thread e ]} ∪ delete i ρ) as HH.
+    { apply map_eq. intro. smap. } rewrite HH.
+    apply pure_holds in Q2 as [[v ->]|Q].
+    + constructor. exists (∅ ∪ delete i ρ).
+      econstructor; last constructor; last solve_map_disjoint.
+      intro x. smap. destruct (_!!x); done.
+    + destruct Q as (k & e0 & [Hk ->] & [[e0' Q] | [[v ->] | [v [j ->]]]]).
+      * constructor. eexists ({[ i := Thread (k e0') ]} ∪ delete i ρ).
+        constructor; [intro j; smap; by destruct (_!!j)..|].
+        constructor; eauto.
+      * constructor.
+        destruct (cfg_fresh2 ρ) as (j & n & Hj & Hn & Hjn).
+        exists ({[ i := Thread (k $ Val $ BarrierV n);
+                   j := Thread (App (Val v) (Val $ BarrierV n));
+                   n := Barrier ]} ∪ delete i ρ).
+        constructor; [intro x; smap; by destruct (_!!x)..|].
+        constructor; eauto; intros ->; simplify_eq.
+      * eapply (Waiting_reachable _ _ j).
+        -- unfold waiting. smap.
+          ++ admit.
+          ++ destruct (ρ !! j) as [[]|] eqn:F; rewrite ?F.
+            ** admit.
+            ** unfold expr_waiting. eauto.
+            ** admit.
+        -- assert (∃ l, out_edges g i !! j = Some l) as [l Hl].
+           { admit. }
+           destruct (IH1 j l).
+           ++ rewrite Hl //.
+           ++ unfold waiting. rewrite E.
+              admit.
+           ++ unfold inactive in H. admit.
+           ++ rewrite -HH //.
+  - eapply affinely_pure_holds in Q as [Q1 [t1 [t2 Q2]]].
 Admitted.
