theories/multiparty/invariant.v
@@ -1255,9 +1255,9 @@ Section invariant.
   Definition invariant (es : list expr) (h : heap) := inv (state_inv es h).
 End invariant.
 
-Instance state_inv_proper es h v : Proper ((≡) ==> (⊣⊢)) (state_inv es h v).
+Global Instance state_inv_proper es h v : Proper ((≡) ==> (⊣⊢)) (state_inv es h v).
 Proof. solve_proper_prepare. destruct v; [solve_proper|by setoid_rewrite H]. Qed.
-Instance state_inv_params : Params (@state_inv) 3. Defined.
+Global Instance state_inv_params : Params (@state_inv) 3. Defined.
 
 Lemma gmap_slice_push `{Countable A,Countable B,Countable C} {V}
     (p : A) (c : B) (q : C) (x : V) (m : bufsT A (B*C) V) :
